A draft of the proof of Kosaraju.

theories/kosaraju.v
@@ -18,12 +18,14 @@ From Stdlib Require Import Uint63.
 From Stdlib Require Import Array.PArray.
 From Stdlib Require Export ZifyNat ZifyUint63.
 From marble Require Import tactics bool int iteration loop array wp.
-From marble.logic Require Import sets relations dfs.
+From marble.logic Require Import sets relations dfs scc.
 From marble Require Import traverse.
 
 Unset Universe Minimization ToSet.
 Generalizable All Variables.
 Set Universe Polymorphism.
+
+Local Ltac wp_intro_hook Hx ::= idtac.
 
 (* -------------------------------------------------------------------------- *)
 
@@ -88,7 +90,6 @@ Variable E : relation vertex.
 
 Local Notation predecessors v := (image (flip E) {[v]}).
 Local Notation successors v   := (image E {[v]}).
-Local Notation closed vs      := (closed E vs).
 Local Notation closure vs     := (closure E vs).
 Local Notation scc v w        := (scc E v w).
 
@@ -141,12 +142,17 @@ Variable wp_foreach_predecessor:
    its strongly connected component. *)
 
 Definition kosaraju : array _vertex :=
-  do vs ← list_rev_post _n (@foreach_vertex) (@foreach_successor) ;
-  let foreach_start {S} (s : S) yield := fold_left yield vs s in
+  do _vs ← list_rev_post _n (@foreach_vertex) (@foreach_successor) ;
+  let foreach_start {S} (s : S) yield := fold_left yield _vs s in
   do _group ← group _n (@foreach_start) (@foreach_predecessor) ;
   _group.
 
 (* -------------------------------------------------------------------------- *)
+
+Implicit Type rs : list vertex.
+Implicit Type vs : vertices.
+
+Context `{!RelDecision (∈@{vertices})}.
 
 Lemma wp_kosaraju :
   wp kosaraju (λ _group,
@@ -157,9 +163,120 @@ Lemma wp_kosaraju :
     (∀ v, 0 ≤ v < n → scc v (ρ !!! v)) ∧
     (* If two vertices [v] and [w] are members of the same component
        then they have the same image through [ρ]. *)
-    (∀ v w, 0 ≤ v < n → 0 ≤ w < n → ρ !!! v = ρ !!! w)
+    (∀ v w, 0 ≤ v < n → 0 ≤ w < n → scc v w → ρ !!! v = ρ !!! w)
   ).
 Proof.
+  unfold kosaraju.
+
+  (* 1a. Definitions. *)
+  set (start := universe n).
+  set (complete := λ rs, list_to_set rs ≡ start).
+
+  (* 1b. Invoke [list_rev_post]. *)
+  specialize (wp_list_rev_post) with
+    (start := start)
+    (complete := complete)
+  ; intro wp_list_rev_post.
+  wp_op wp_list_rev_post introducing: _vs; clear wp_list_rev_post.
+  (* Precondition 1: the predicate [complete] is inhabited. *)
+  { apply finite_universe. }
+  (* Precondition 2: *)
+  (* We must prove that the specification of [foreach_vertex], which
+     is formulated using [ITER_SET], implies a formulation that is
+     formulated directly in terms of [ITER] and [complete]. This is
+     essentially the same proof as the lemma [misc.direction1]. *)
+  (* TODO make this a separate lemma *)
+  { clear -wp_foreach_vertex.
+    intros. ITER.
+    wp_op wp_foreach_vertex with invariant: (
+      λ vs s, ∃ rs, inv rs s ∧ list_to_set rs ≡ vs
+    ).
+    (* Compatibility. *)
+    { clear dependent s.
+      intros vs1 vs2 Hequiv. intros s ? <-.
+      split; intros; unpack; pack; eauto; set_solver. }
+    (* Initialization. *)
+    { pack; eauto. }
+    (* Preservation. *)
+    { clear dependent s.
+      intros vs0 vs1 s (rs & ? & ?).
+      intros v _ ? ? _v ?.
+      wp_op Hbody shadowing: s.
+      { unfold permitted, complete.
+        (* We must argue that the set [universe n ∖ vs1] is finite. *)
+        destruct (finite_universe n) as (rs' & Hcover).
+        exists rs'. set_solver. }
+      eexists. split. eauto. set_solver.
+    }
+    (* Completion. *)
+    { clear dependent s.
+      intros s (vs & (rs & ? & ?) & ?).
+      unfold complete, universe.
+      eexists. split. eauto. set_solver. }
+  }
+
+  (* 1c. Deconstruct the postcondition of [list_rev_post]. *)
+  match goal with Hpost: _ |- _ =>
+    destruct Hpost as (marked & f1 & Hdfs1 & Hroots & Hmarked & Hvs)
+  end. (* TODO tactic *)
+  (* Every vertex is marked. *)
+  rewrite (closure_start_is_universe n start) in Hmarked by eauto with lia.
+  rewrite Hmarked in Hdfs1.
+  (* The list [_vs] corresponds to [vs], a reverse postorder enumeration
+     of the forest [f1]. *)
+  set (vs := rev (postorder f1)). fold vs in Hvs.
+  clear dependent marked.
+  clear Hroots. (* unused *)
+  (* The universe is reverse closed. *)
+  assert (closed (flip E) (universe n)) by set_solver.
+
+  (* 2a. More definitions. *)
+  (* This time, the predicate [complete] is deterministic: it is important
+     that the root vertices be enumerated in the order of the list [vs]. *)
+  clear complete.
+  set (complete := λ rs, rs = vs).
+
+  (* 2b. Invoke [group]. *)
+  specialize (wp_group _n n isInt_n bound_n) with
+    (start := start)
+    (complete := complete)
+    (E := flip E)
+    (wp_foreach_successor := @wp_foreach_predecessor)
+  ; intro wp_group.
+  wp_op wp_group introducing: _group; clear wp_group.
+  (* Precondition 1: the list [vs] covers the set [start]. *)
+  { unfold complete. intros ? ->.
+    subst vs. rewrite list_to_set_rev, list_to_set_postorder.
+    dfs_omarked. apply dfs_omarked_choice in Hdfs1. set_solver. }
+  (* Precondition 2: the predicate [complete] is inhabited. *)
+  { unfold complete. eauto. }
+  (* Precondition 3: [fold_left _ _vs _] enumerates the list [vs]. *)
+  { admit. } (* TODO create a file list.v *)
+
+  (* 2c. Deconstruct the postcondition of [group]. *)
+  match goal with Hpost: _ |- _ => destruct Hpost as
+    (marked & f2 & ρ & Hdfs2 & Hroots & ? & Hgroup & ? & Hmap)
+  end. (* TODO make this a tactic *)
+
+  assert (Hmarked: marked ≡ closure start) by admit. (* TODO wp_group could give this *)
+  (* Every vertex is marked. *)
+  rewrite (closure_start_is_universe n start) in Hmarked by eauto with lia.
+  rewrite Hmarked in Hdfs2.
+  clear dependent marked.
+  clear Hroots. (* unused *)
+
+  assert (ordered vs f2). (* TODO missing in the spec of [group]? *)
+  admit.
+
+  (* 3. Conclude. *)
+  assert (is_scc_forest E f2).
+  { eapply scc_soundness. econstructor. eauto. }
+  wp_ret. eexists; pack; tc.
+  (* Postcondition 1: [v] and [ρ !!! v] inhabit the same component. *)
+  { admit. }
+  (* Postcondition 2: if [v] and [w] inhabit the same component then
+     [ρ !!! v] and [ρ !!! w] are equal. *)
+  { admit. }
 Abort.
 
 End G.
